Initial working version done with Jasmin

untyped_arithmetic_expressions.thy
@@ -11,11 +11,6 @@ inductive is_value :: "B_term \<Rightarrow> bool" where
   "is_value BTrue" |
   "is_value BFalse"
 
-thm is_value.induct
-thm is_value.intros
-thm is_value.cases
-thm is_value.simps
-
 inductive_cases is_value_BIfD: "is_value (BIf t1 t2 t3)"
 
 inductive eval_once :: "B_term \<Rightarrow> B_term \<Rightarrow> bool" where
@@ -23,16 +18,58 @@ inductive eval_once :: "B_term \<Rightarrow> B_term \<Rightarrow> bool" where
   e_if_false: "eval_once (BIf BFalse t2 t3) t3" |
   e_if: "eval_once t1 t1' \<Longrightarrow> eval_once (BIf t1 t2 t3) (BIf t1' t2 t3)"
 
-thm eval_once.induct
-thm eval_once.intros
-thm eval_once.cases
-thm eval_once.simps
-
 inductive_cases eval_once_BTrueD: "eval_once BTrue t"
 inductive_cases eval_once_BFalseD: "eval_once BFalse t"
 
+inductive eval :: "B_term \<Rightarrow> B_term \<Rightarrow> bool" where
+  e_once: "eval_once t t' \<Longrightarrow> eval t t'" |
+  e_self: "eval t t" |
+  e_transitive: "eval t t' \<Longrightarrow> eval t' t'' \<Longrightarrow> eval t t''"
+
+inductive eval' :: "B_term \<Rightarrow> B_term \<Rightarrow> bool" where
+  e_base': "eval' t t" |
+  e_step': "eval_once t t' \<Longrightarrow> eval' t' t'' \<Longrightarrow> eval' t t''"
+
+lemma e_once': "eval_once t t' \<Longrightarrow> eval' t t'"
+  by (simp add: e_base' e_step')
+
+lemma e_transitive': "eval' t t' \<Longrightarrow> eval' t' t'' \<Longrightarrow> eval' t t''"
+  using assms proof (induction t t' arbitrary: t'' rule: eval'.induct)
+    case (e_base' t t'') thus ?case .
+  next
+    case (e_step' t t' t'' t''')
+    thus ?case
+      using eval'.e_step' by blast
+  qed
+
+lemma eval_eq_eval': "eval = eval'"
+  apply (rule ext)+
+  apply (rule iffI)
+   apply (rename_tac t t')
+   apply (erule eval.induct)
+      apply (erule e_once')
+    apply (rule e_base')
+   apply (erule e_transitive')
+   apply assumption
+  apply (erule eval'.induct)
+   apply (rule e_self)
+  using e_once e_transitive by blast
+
 inductive is_normal_form :: "B_term \<Rightarrow> bool" where
   "\<forall>t'. \<not> eval_once t t' \<Longrightarrow> is_normal_form t"
+
+(*
+definition is_normal :: "B_term \<Rightarrow> bool" where
+  "is_normal t \<longleftrightarrow> (\<forall>t'. \<not> eval_once t t')"
+*)
+
+inductive_cases is_normal_form_BIfD: "is_normal_form (BIf t1 t2 t3)"
+
+lemma is_normal_form_BTrue: "is_normal_form BTrue"
+  using eval_once_BTrueD is_normal_form.intros by blast
+
+lemma is_normal_form_BFalse: "is_normal_form BFalse"
+  using eval_once_BFalseD is_normal_form.intros by blast
 
 lemma
   assumes
@@ -55,9 +92,8 @@ lemma not_eval_once_BTrue: "\<not> eval_once BTrue t"
 lemma not_eval_once_BFalse: "\<not> eval_once BFalse t"
   by (blast dest: eval_once_BFalseD)
 
-lemma
-  fixes
-    t t' t'' :: B_term
+theorem eval_single_determinacy:
+  fixes t t' t'' :: B_term
   shows "eval_once t t' \<Longrightarrow> eval_once t t'' \<Longrightarrow> t' = t''"
 proof (induction t t' arbitrary: t'' rule: eval_once.induct)
   case (e_if_true t1 t2)
@@ -97,5 +133,85 @@ proof (rule ccontr, induction t rule: B_term.induct)
     case (BIf t1 t2 t3)
     thus ?case by (metis e_if e_if_false e_if_true is_normal_form.cases is_normal_form.intros is_value.cases)
 qed
+
+corollary
+  fixes t u u' :: B_term
+  assumes
+    "eval t u" and
+    "eval t u'" and
+    "is_normal_form u" and
+    "is_normal_form u'"
+  shows "u = u'"
+using assms
+unfolding eval_eq_eval'
+proof (induction t u rule: eval'.induct)
+  case (e_base' t)
+  thus ?case
+    by (metis eval'.cases is_normal_form.cases)
+next
+  case (e_step' t t' t'')
+  thus ?case
+    by (metis eval'.cases is_normal_form.cases eval_single_determinacy)
+qed
+
+
+primrec size_B :: "B_term \<Rightarrow> nat" where
+  "size_B BTrue = 1" |
+  "size_B BFalse = 1" |
+  "size_B (BIf t1 t2 t3) = size_B t1 + size_B t2 + size_B t3"
+
+lemma size_B_nz[simp]: "size_B t \<noteq> 0"
+  by (induct t) auto
+
+lemma eval_once_size_B:
+  assumes "eval_once t t'"
+  shows "size_B t > size_B t'"
+using assms
+proof (induction rule: eval_once.induct)
+  case e_if_true thus ?case by simp
+next
+  case e_if_false thus ?case by simp
+next
+  case e_if thus ?case by simp
+qed
+
+
+thm less_induct
+thm Nat.measure_induct_rule
+
+theorem "\<exists>t'. eval t t' \<and> is_normal_form t'"
+  unfolding eval_eq_eval'
+  apply (induct rule: measure_induct_rule[of size_B])
+  apply (rename_tac t)
+  apply (case_tac "is_normal_form t")
+  apply (rule_tac x = t in exI)
+  apply (rule conjI)
+  apply (rule e_base')
+  apply assumption
+  apply (subst (asm) (2) is_normal_form.simps[simplified])
+  apply simp
+  apply (erule exE)
+  using e_step' eval_once_size_B by blast
+
+find_theorems "\<not> (\<forall>x. _)"
+
+
+theorem "\<exists>t'. eval t t' \<and> is_normal_form t'"
+proof (induction t)
+  case BTrue
+  thus ?case using e_self is_normal_form_BTrue by auto
+next
+  case BFalse
+  thus ?case using e_self is_normal_form_BFalse by auto
+next
+  case (BIf t1 t2 t3)
+  thus ?case
+  apply (cases t1)
+    using e_if_true e_once e_transitive apply blast
+   using e_if_false e_once e_transitive apply blast
+   apply hypsubst
+   apply auto
+qed
+
 
 end
